cleanup1

ExistentialRules/ChaseSequence/CoreChase/Core.lean
@@ -17,57 +17,11 @@ import ExistentialRules.ChaseSequence.CoreChase.Triggers
 import ExistentialRules.ChaseSequence.CoreChase.Termination
 
 
---import ExistentialRules.BasicTypes.Sets.Set
---import ExistentialRules.BasicTypes.Sets.Finite
---import ExistentialRules.BasicTypes.Functions.Function
-
-
---import Aesop
--- import Canonical
--- import Mathlib.Combinatorics.Graph.Basic
-
-
--- set_option pp.proofs true
--- set_option diagnostics true
-
 variable {sig : Signature} [DecidableEq sig.P] [DecidableEq sig.C] [DecidableEq sig.V]
 variable {kb : KnowledgeBase sig}
---abbrev obs := RestrictedObsolescence sig
 
 
 namespace CoreChaseBranch
-
-
-  abbrev InductiveHomomorphismResultCore (cb : CoreChaseBranch kb) (m : FactSet sig) (depth : Nat) :=
-    {gtm : GroundTermMapping sig // ∀ cn, cn ∈ cb.branch.get? depth → gtm.isHomomorphism cn.fs m}
-
-
-  @[grind .]
-  theorem kb_det_head_len_eq (kb_det : kb.isDeterministic): ∀ (r : Rule sig), r ∈ kb.rules.rules → r.head.length = 1 := by
-    unfold KnowledgeBase.isDeterministic RuleSet.isDeterministic Rule.isDeterministic at kb_det
-    intro r r_in
-    specialize kb_det r r_in
-    grind
-
-  theorem func_term_not_mem_head {cb : CoreChaseBranch kb} {t : GroundTerm sig} (t_is_func : ∃ func ts arity_ok, t = GroundTerm.func func ts arity_ok) :
-    ¬ t ∈ cb.head.fs.terms := by
-      intro t_mem
-      rcases t_mem with ⟨f, f_mem, t_mem⟩
-      rcases kb.db.toFactSet.property.right f (by grind) t t_mem with ⟨c, t_eq⟩
-      rcases t_is_func with ⟨_, _, _, t_eq'⟩
-      rw [t_eq'] at t_eq
-      simp [GroundTerm.func_neq_const] at t_eq
-
-
-theorem ex_endo_hom  (cb : CoreChaseBranch kb) (cn : CoreChaseNode kb.rules)
-    (disj_idx n : Nat) (trg: RTrigger obs.toLaxObsolescenceCondition kb.rules) (cn_eq : cn ∈ cb.branch.get? n)
-    (t : GroundTerm sig ) (lt : disj_idx < trg.val.rule.head.length)
-    (t_mem_trg : t ∈ trg.val.fresh_terms_for_head_disjunct disj_idx lt) (t_mem_node : t ∈ cn.fs.terms) :
-      ∃ (gtm : GroundTermMapping sig), gtm.isHomomorphism (trg.val.mapped_head[disj_idx]'(by rw [PreTrigger.length_mapped_head]; exact lt)).toSet cn.core ∧
-        gtm.isHomomorphism cn.core cn.core ∧ (Function.surjective_for_domain_and_image_set gtm cn.core.terms cn.core.terms) := by
-          have : trg.val.satisfied_for_disj cn.fs ⟨disj_idx, Nat.lt_of_succ_le lt⟩ := by
-            sorry
-          sorry
 
   -- jeder surjektive endomorphisms auf endlichen mengen ist auch ein isomorphismus
 
@@ -82,315 +36,6 @@ theorem ex_endo_hom  (cb : CoreChaseBranch kb) (cn : CoreChaseNode kb.rules)
 
 
 
-  --set_option trace.Meta.synthInstance true
-  noncomputable def inductive_homomorphism_core_with_prev_node_and_trg_if_next_node_some (cb : CoreChaseBranch kb) (m : FactSet sig) (m_mod : m.modelsKb kb) (kb_det : kb.isDeterministic)
-    (prev_depth : Nat) (prev_node : CoreChaseNode kb.rules) (prev_node_eq : prev_node ∈ cb.branch.get? prev_depth)
-    (prev_gtm : GroundTermMapping sig) (prev_gtm_hom : prev_gtm.isHomomorphism prev_node.fs m) :
-      ∀ next_node ∈ cb.branch.get? (prev_depth.succ), ∃ (next_gtm : GroundTermMapping sig), GroundTermMapping.isHomomorphism next_gtm next_node.fs m := by
-
-        intro next_node next_node_eq
-
-        have prev_core_eq : (cb.prev_node prev_depth (Option.isSome_of_mem next_node_eq)).core = prev_node.core := by grind
-
-        have prev_gtm_hom_core : prev_gtm.isHomomorphism prev_node.core m := homFsToFsAlsoHomCoreToFs m prev_node prev_gtm prev_gtm_hom
-
-        have trg_act := cb.triggers_active prev_depth prev_node prev_node_eq next_node next_node_eq
-
-        let trg_on_prev_node := (Classical.choose trg_act).fst -- origin.fst
-        let disj_on_prev_node := (Classical.choose trg_act).snd --origin.snd
-
-        let fin_disj : Fin trg_on_prev_node.val.rule.head.length :=
-            ⟨disj_on_prev_node.val, by
-              rw [← PreTrigger.length_mapped_head]
-              exact disj_on_prev_node.isLt
-              ⟩
-
-        let trg_active_prev_core := (Classical.choose_spec trg_act).right
-
-        let next_node_origin_some := (Classical.choose_spec trg_act).left
-
-        let next_node_origin := next_node.origin.get (origin_isSome cb prev_depth next_node_eq)
-
-
-        let new_trg : PreTrigger sig := ⟨trg_on_prev_node.val.rule, (prev_gtm ∘ trg_on_prev_node.val.subs)⟩
-
-        have new_trg_loaded : new_trg.loaded m := by
-          apply Set.subset_trans _ prev_gtm_hom.right
-          apply PreTrigger.term_mapping_preserves_loadedness
-          . exact prev_gtm_hom.left
-          . have trg_origin_act := (cb.origin_trg_is_active_prev_core prev_depth next_node next_node_eq ⟨trg_on_prev_node, disj_on_prev_node⟩ next_node_origin_some).left
-            simp [prev_core_eq] at trg_origin_act
-            have := trg_loaded_in_fs_if_loaded_in_core cb prev_depth prev_node prev_node_eq trg_on_prev_node.val trg_origin_act
-            exact this
-
-
-        have new_trg_satisfied : new_trg.satisfied_for_disj m ⟨fin_disj.val, fin_disj.isLt⟩ := by
-          have modelsRule : m.modelsRule new_trg.rule := m_mod.right new_trg.rule trg_on_prev_node.property
-          unfold FactSet.modelsRule at modelsRule
-          specialize modelsRule new_trg.subs new_trg_loaded
-
-          rcases modelsRule with ⟨i, s', s'_frontier, s'_contains⟩
-          exists s'
-          constructor
-          . exact s'_frontier
-          . have : i.val = fin_disj.val := by
-              have isLt := i.isLt
-              have := kb_det new_trg.rule trg_on_prev_node.property
-              unfold Rule.isDeterministic at this
-              rw [decide_eq_true_iff] at this
-              simp only [this, Nat.lt_one_iff] at isLt
-              have isLt' := fin_disj.isLt
-              have := kb_det trg_on_prev_node.val.rule trg_on_prev_node.property
-              unfold Rule.isDeterministic at this
-              rw [decide_eq_true_iff] at this
-              simp only [this, Nat.lt_one_iff] at isLt'
-              rw [isLt, isLt']
-            simp only [List.get_eq_getElem, this] at s'_contains
-            exact s'_contains
-
-        let subs := Classical.choose new_trg_satisfied
-        have ⟨subs_frontier, subs_contained⟩ := Classical.choose_spec new_trg_satisfied
-
-        -- build new hom
-        let next_gtm : GroundTermMapping sig := fun t =>
-          if t_mem : t ∈ (trg_on_prev_node.val.fresh_terms_for_head_disjunct ↑fin_disj fin_disj.isLt) then
-            subs (trg_on_prev_node.val.existential_var_for_fresh_term ↑fin_disj fin_disj.isLt t t_mem)
-          else
-            prev_gtm t
-
-        have next_gtm_is_id_on_const : next_gtm.isIdOnConstants := by
-          intro c
-          have : ¬ GroundTerm.const c ∈ trg_on_prev_node.val.fresh_terms_for_head_disjunct ↑fin_disj fin_disj.isLt := by
-            apply PreTrigger.constant_not_mem_fresh_terms_for_head_disjunct
-          simp_all
-          simp only [next_gtm, this, ↓reduceDIte]
-          exact prev_gtm_hom.left
-
-
-        have next_gtm_is_subs_on_head_vars : ∀ v, v ∈ (trg_on_prev_node.val.rule.head[fin_disj.val]).vars -> (next_gtm (trg_on_prev_node.val.subs_for_mapped_head disj_on_prev_node v)) = subs v := by
-          intro v v_mem
-          simp only [PreTrigger.subs_for_mapped_head]
-          cases Decidable.em (v ∈ trg_on_prev_node.val.rule.frontier) with
-          | inl v_frontier =>
-            rw [trg_on_prev_node.val.apply_to_var_or_const_frontier_var _ _ v_frontier]
-            have : ¬ trg_on_prev_node.val.subs v ∈ trg_on_prev_node.val.fresh_terms_for_head_disjunct fin_disj.val fin_disj.isLt := by
-              apply PreTrigger.frontier_term_not_mem_fresh_terms_for_head_disjunct
-              apply List.mem_map_of_mem
-              exact v_frontier
-            simp only [next_gtm, this, ↓reduceDIte]
-            simp only [subs, subs_frontier _ v_frontier]
-            rfl
-          | inr v_frontier =>
-            rw [trg_on_prev_node.val.apply_to_var_or_const_non_frontier_var _ _ v_frontier]
-            have v_exis : v ∈ trg_on_prev_node.val.rule.existential_vars_for_head_disjunct fin_disj.val fin_disj.isLt := by
-              simp only [Rule.existential_vars_for_head_disjunct, List.mem_filter, decide_eq_true_iff]
-              exact ⟨v_mem, v_frontier⟩
-            have : trg_on_prev_node.val.functional_term_for_var disj_on_prev_node.val v ∈ trg_on_prev_node.val.fresh_terms_for_head_disjunct fin_disj.val fin_disj.isLt := by
-              apply List.mem_map_of_mem; exact v_exis
-            simp only [next_gtm, this, ↓reduceDIte]
-            rw [PreTrigger.existential_var_for_fresh_term_after_functional_term_for_var]
-            exact v_exis
-
-        have next_gtm_eq_prev_gtm_on_terms_in_prev_node : ∀ t ∈ prev_node.core.terms, next_gtm t = prev_gtm t := by
-          intro t t_mem
-          have n_eq : (cb.prev_node prev_depth (Option.isSome_of_mem next_node_eq)) = prev_node := by grind
-
-          have : ¬ t ∈ trg_on_prev_node.val.fresh_terms_for_head_disjunct fin_disj.val fin_disj.isLt := by
-            intro contra
-            apply trg_active_prev_core.right
-
-            apply obs.contains_trg_result_implies_cond disj_on_prev_node
-
-            intro f f_mem
-
-            have ex_gtm := cb.result_of_trigger_introducing_functional_term_occurs_in_chase_core' prev_node disj_on_prev_node prev_depth (Classical.choose trg_act).fst
-              (Option.mem_def.mpr prev_node_eq) t fin_disj.isLt (by grind) (CoreChaseNode.fs_terms_sub_core_terms prev_node t t_mem)
-
-            have := CoreChaseBranch.functional_term_originates_from_some_trigger_or_database_core cb prev_depth prev_node prev_node_eq t
-              (PreTrigger.term_functional_of_mem_fresh_terms t contra) (CoreChaseNode.fs_terms_sub_core_terms prev_node t t_mem)
-
-            cases this with
-              | inl from_db =>
-                have := func_term_not_mem_head (PreTrigger.term_functional_of_mem_fresh_terms t contra) from_db
-                contradiction
-              | inr from_trg =>
-                rcases ex_gtm with ⟨gtm, gtm_idc, gtm_af⟩
-
-                have : f ∈ gtm.applyFactSet (Classical.choose trg_act).fst.val.mapped_head[↑disj_on_prev_node].toSet := by
-                  unfold GroundTermMapping.applyFactSet
-                  rw [GroundTermMapping.mem_applyFactSet]
-                  exists f
-                  constructor
-                  exact List.mem_toSet.mpr f_mem
-                  specialize gtm_af (gtm.applyFact f)
-                    (TermMapping.apply_generalized_atom_mem_apply_generalized_atom_set gtm f (Classical.choose trg_act).fst.val.mapped_head[↑disj_on_prev_node].toSet f_mem)
-                  rcases from_trg with ⟨m, cm, cm_eq, cm_o, cm_o_eq, h⟩
-
-                  have ex_endo := ex_endo_hom cb prev_node disj_on_prev_node prev_depth trg_on_prev_node prev_node_eq
-                    t fin_disj.isLt (by grind) (CoreChaseNode.fs_terms_sub_core_terms prev_node t t_mem)
-
-                  rcases ex_endo with ⟨gtm_endo, gtm_endo_hom, gtm_endo_endo, gtm_endo_surj⟩
-
-
-                  have ex_eq_list : ∃ (tl : List (GroundTerm sig)), tl.toSet = prev_node.core.terms := by
-                    have := Set.exListOfSetIfFin prev_node.core.terms (by
-                      have := CoreChaseNode.all_core_finite prev_node
-                      exact FactSet.terms_finite_of_finite prev_node.core this
-                      )
-                    rcases this with ⟨l, l_eq⟩
-                    exists l
-                    exact Set.ext l.toSet prev_node.core.terms l_eq
-
-                  rcases ex_eq_list with ⟨tl, tl_eq⟩
-
-                  have gtm_surj_list : Function.surjective_for_domain_and_image_list gtm_endo tl tl := by
-
-                    unfold Function.surjective_for_domain_and_image_list
-                    intro b b_in
-                    exists b
-                    constructor
-                    exact b_in
-                    have : b ∈ prev_node.core.terms := by grind
-                    have : ∃ g, g ∈ prev_node.core ∧ b ∈ g.terms := Exists.imp (fun a a_1 => a_1) this
-                    rcases this with ⟨g, g_in, g_term_in⟩
-                    sorry
-
-                  have ex_reps := gtm_endo.exists_repetition_that_is_inverse_of_surj tl gtm_surj_list
-
-                  rcases ex_reps with ⟨k_rep, h_rep⟩
-                  specialize h_rep t (by grind)
-
-
-                  sorry
-
-                specialize gtm_af f this
-                exact gtm_af
-
-          simp [next_gtm, this]
-
-        exists next_gtm
-
-        constructor
-        · exact next_gtm_is_id_on_const
-        · intro f'
-          rw [GroundTermMapping.mem_applyFactSet]
-          intro ⟨f, f_mem, f'_eq⟩
-          rw [cb.origin_trg_result_yields_next_node_fs prev_depth next_node next_node_eq] at f_mem
-          rw [f'_eq]
-          cases f_mem with
-            -- f comes from prev core
-            | inl f_mem =>
-              apply prev_gtm_hom.right
-              rw [GroundTermMapping.mem_applyFactSet]
-              exists f
-              constructor
-              · exact prev_node.core_sse.left f (by rw [prev_core_eq] at f_mem; exact f_mem)
-              · apply TermMapping.apply_generalized_atom_congr_left
-                intro t t_mem
-                apply next_gtm_eq_prev_gtm_on_terms_in_prev_node
-                exists f
-                grind
-            -- f comes from trg result
-            | inr f_mem =>
-              apply subs_contained
-              have : (subs.apply_function_free_conj new_trg.rule.head[fin_disj.val]).toSet = next_gtm.applyFactSet trg_on_prev_node.val.mapped_head[↑fin_disj].toSet := by
-                simp only [TermMapping.apply_generalized_atom_set_toSet]
-                apply congrArg
-                simp only [Fin.getElem_fin]
-                rw [← PreTrigger.apply_subs_for_mapped_head_eq, ← GroundSubstitution.apply_function_free_conj_compose]
-                . apply List.map_congr_left
-                  intro a a_mem
-                  apply TermMapping.apply_generalized_atom_congr_left
-                  intro voc voc_mem
-                  cases voc with
-                  | const d => simp [GroundSubstitution.apply_var_or_const]
-                  | var v =>
-                    simp only [GroundSubstitution.apply_var_or_const, Function.comp_apply]
-                    rw [next_gtm_is_subs_on_head_vars]
-                    rw [FunctionFreeConjunction.mem_vars]
-                    exists a
-                . intros; exact next_gtm_is_id_on_const
-              rw [this]
-              apply TermMapping.apply_generalized_atom_mem_apply_generalized_atom_set
-              simp [CoreChaseNode.origin_result] at f_mem
-              have n_eq : (cb.prev_node prev_depth (Option.isSome_of_mem next_node_eq)) = prev_node := by grind
-              have eq2 : (next_node.origin.get (origin_isSome cb prev_depth next_node_eq)).fst = trg_on_prev_node := by sorry
-              have eq3 : (next_node.origin.get (origin_isSome cb prev_depth next_node_eq)).snd.val = disj_on_prev_node := by sorry
-              simp only [eq2, eq3] at f_mem
-              exact f_mem
-
-
-  noncomputable def inductive_homomorphism_core (cb : CoreChaseBranch kb) (m : FactSet sig) (m_mod : m.modelsKb  kb) (kb_det : kb.isDeterministic) : (depth : Nat) → InductiveHomomorphismResultCore cb m depth
-      | .zero => ⟨id, by
-        intro cn cn_eq
-        rw [cb.database_first] at cn_eq
-        constructor
-        · intro c; rfl
-        · intro f f_in
-          apply m_mod.left
-          rw [Option.mem_some] at cn_eq
-          simp only [FactSet.applyFactSetIdEq, ← cn_eq] at f_in
-          exact f_in
-      ⟩
-
-      | .succ j =>
-        let prev_gtm := (inductive_homomorphism_core cb m m_mod kb_det j).val
-        let prev_gtm_hom := (inductive_homomorphism_core cb m m_mod kb_det j).property
-        let prev_node := cb.branch.infinite_list j
-
-        match prev_node_eq : prev_node with
-          | .none => ⟨prev_gtm, by
-            intro cn cn_eq
-            rw [none_get_eq] at prev_node_eq
-            have := @PossiblyInfiniteList.no_holes' _ cb.branch j prev_node_eq
-            rw [Option.mem_def, this] at cn_eq
-            contradiction
-              ⟩
-          | .some cn =>
-            match c1 : Classical.propDecidable (∃ (trg : RTrigger obs.toLaxObsolescenceCondition kb.rules), trg.val.active (prev_node.get (Option.isSome_of_mem prev_node_eq)).core) with
-              | isTrue tr =>
-                let trg := Classical.choose tr
-                let trg_act := Classical.choose_spec tr
-                have ex_next_node := exNextNodeIfExActiveTrigger cb j cn prev_node_eq trg (by grind)
-                let next_node := Classical.choose ex_next_node
-                let next_node_eq := Classical.choose_spec ex_next_node
-                have := inductive_homomorphism_core_with_prev_node_and_trg_if_next_node_some
-                  cb m m_mod kb_det j cn prev_node_eq prev_gtm (GroundTermMapping.subPreservesHom cn.fs m cn.fs (Set.subset_refl) prev_gtm (prev_gtm_hom cn prev_node_eq)) next_node next_node_eq
-                let next_gtm := Classical.choose this
-                have next_gtm_hom := Classical.choose_spec this
-                ⟨next_gtm, by
-                  intro cn' cn'_eq
-                  have : cn' = next_node := mem_eq cb cn' next_node j.succ cn'_eq next_node_eq
-                  subst next_gtm this
-                  exact next_gtm_hom
-                  ⟩
-              | isFalse fa =>
-                ⟨prev_gtm, by
-                  intro cn' cn'_eq
-                  have t := prev_gtm_hom cn prev_node_eq
-                  simp only [not_exists] at fa
-                  have next_none : (cb.branch.get? j.succ) = none := by
-                    have := cb.no_succ_chase_node_if_not_exists_active_trigger_core cn j (Option.mem_def.mpr prev_node_eq) (by grind)
-                    exact Option.isNone_iff_eq_none.mp this
-                  rw [next_none] at cn'_eq
-                  contradiction
-                  ⟩
-
-
-
-  theorem coreChaseResultIsUniversal (cb : CoreChaseBranch kb) (ter' : cb.terminates') (kb_det : kb.isDeterministic) : ∀ (m : FactSet sig), m.modelsKb kb → ∃ (h : GroundTermMapping sig), h.isHomomorphism (cb.result ter') m := by
-    intro m m_mod
-    let result : FactSet sig := cb.result ter'
-    rcases ter' with ⟨n_ter, is_some, is_none⟩
-    let h:= inductive_homomorphism_core cb m m_mod kb_det n_ter
-    exists h
-    have p := h.property
-    unfold CoreChaseBranch.result
-    have : ∃ cn_res, cb.branch.infinite_list n_ter = some cn_res := Option.ne_none_iff_exists'.mp is_some
-    rcases this with ⟨cn_res, cn_res_eq⟩
-    specialize p cn_res cn_res_eq
-    have := homFsToFsAlsoHomCoreToFs m cn_res h.val p
-    grind
 
   -- main theorem
   -- if cb.terminates → cb.result.universalmodels kb ∧ Set.finite cb.result
@@ -663,7 +308,7 @@ theorem ex_endo_hom  (cb : CoreChaseBranch kb) (cn : CoreChaseNode kb.rules)
     rcases S_fin with ⟨l, l_nd, l_eq⟩
     exists l
 
-  noncomputable def generateNextCoreChaseBranchElement (o : (trg : RTrigger obs.toLaxObsolescenceCondition kb.rules) × Fin trg.val.mapped_head.length) (last_node : CoreChaseNode kb.rules) : CoreChaseNode kb.rules :=
+  noncomputable def generateNextCoreChaseBranchElement' (o : (trg : RTrigger obs.toLaxObsolescenceCondition kb.rules) × Fin trg.val.mapped_head.length) (last_node : CoreChaseNode kb.rules) : CoreChaseNode kb.rules :=
 
 
     let trg_result : FactSet sig := (o.fst.val.mapped_head[o.snd]).toSet
@@ -699,7 +344,7 @@ theorem ex_endo_hom  (cb : CoreChaseBranch kb) (cn : CoreChaseNode kb.rules)
 
     -- generator from node to succ node
 
-    noncomputable def generateNextCoreChaseBranchElement_usingTrigger (ccn : CoreChaseNode kb.rules) (o : (trg : RTrigger obs.toLaxObsolescenceCondition kb.rules) × Fin trg.val.mapped_head.length) : CoreChaseNode kb.rules :=
+    noncomputable def generateNextCoreChaseBranchElement (ccn : CoreChaseNode kb.rules) (o : (trg : RTrigger obs.toLaxObsolescenceCondition kb.rules) × Fin trg.val.mapped_head.length) : CoreChaseNode kb.rules :=
 
       let trg_result : FactSet sig := (o.fst.val.mapped_head[o.snd]).toSet
 
@@ -729,17 +374,28 @@ theorem ex_endo_hom  (cb : CoreChaseBranch kb) (cn : CoreChaseNode kb.rules)
     ccn_succ
 
 
-  noncomputable def generateNextCoreChaseBranchElement_usingTrigger_only_active_opt (ccn : CoreChaseNode kb.rules) (o : (trg : RTrigger obs.toLaxObsolescenceCondition kb.rules) × Fin trg.val.mapped_head.length) : Option (CoreChaseNode kb.rules) :=
+  noncomputable def generateNextCoreChaseBranchElement_opt (ccn : CoreChaseNode kb.rules) (o : (trg : RTrigger obs.toLaxObsolescenceCondition kb.rules) × Fin trg.val.mapped_head.length) : Option (CoreChaseNode kb.rules) :=
     match Classical.propDecidable (o.fst.val.active ccn.core) with
       | isTrue _ =>
-        generateNextCoreChaseBranchElement_usingTrigger ccn o
+        generateNextCoreChaseBranchElement ccn o
       | isFalse _ =>
         none
 
 
+  def κ (nl : PossiblyInfiniteList (CoreChaseNode kb.rules)) (n : Nat) : Nat :=
+    match n with
+      | .zero => 0
+      | .succ n =>
+        match nl.get? (κ nl n) with
+          | none => κ nl n
+          | some cn =>
+
+
+
+
   theorem exists_active_trigger_of_step [DecidableEq β] (origin_list : List ((trg : RTrigger obs.toLaxObsolescenceCondition kb.rules) × Fin trg.val.mapped_head.length))
     (init_ccn : CoreChaseNode kb.rules) (node_list : (List (CoreChaseNode kb.rules × Option ((trg : RTrigger obs.toLaxObsolescenceCondition kb.rules) × Fin trg.val.mapped_head.length))))
-    (node_list_eq : node_list = foldl_save_hist_opt_nodup_trace origin_list init_ccn generateNextCoreChaseBranchElement_usingTrigger_only_active_opt)
+    (node_list_eq : node_list = foldl_save_hist_opt_nodup_trace origin_list init_ccn generateNextCoreChaseBranchElement_opt)
     (n : Nat) (h : n + 1 < node_list.length) (before after : CoreChaseNode kb.rules)
     (before_eq : before = (node_list.get ⟨n, (Nat.lt_of_succ_lt h)⟩).fst) (after_eq : after = (node_list.get ⟨n+1, Nat.lt_of_succ_le h⟩).fst) (origin_some : after.origin ≠ none) :
       (after.origin.get (Option.isSome_iff_ne_none.mpr origin_some)).fst.val.active before.core := by
@@ -748,7 +404,7 @@ theorem ex_endo_hom  (cb : CoreChaseBranch kb) (cn : CoreChaseNode kb.rules)
 
         have hstep : after ≠ before := by
           have := foldl_save_hist_opt_nodup_trace_adjacent_ne
-            origin_list init_ccn generateNextCoreChaseBranchElement_usingTrigger_only_active_opt n
+            origin_list init_ccn generateNextCoreChaseBranchElement_opt n
             (Nat.lt_of_lt_of_eq h (congrArg List.length node_list_eq))
           subst node_list_eq after_eq before_eq
           -- because nodup
@@ -756,11 +412,11 @@ theorem ex_endo_hom  (cb : CoreChaseBranch kb) (cn : CoreChaseNode kb.rules)
 
         have hex :
           ∃ o ∈ origin_list,
-            generateNextCoreChaseBranchElement_usingTrigger_only_active_opt before o = some after := by sorry
+            generateNextCoreChaseBranchElement_opt before o = some after := by sorry
 
         rcases hex with ⟨o, ho_mem, hgen⟩
 
-        unfold generateNextCoreChaseBranchElement_usingTrigger_only_active_opt at hgen
+        unfold generateNextCoreChaseBranchElement_opt at hgen
 
         cases hdec :
           Classical.propDecidable ((after.origin.get (Option.isSome_iff_ne_none.mpr origin_some)).fst.val.active before.core) with
@@ -775,8 +431,10 @@ theorem ex_endo_hom  (cb : CoreChaseBranch kb) (cn : CoreChaseNode kb.rules)
 
   noncomputable def buildCoreChaseBranchFromChaseBranch (scb : ChaseBranch obs kb) (scb_term : scb.terminates) : CoreChaseBranch kb :=
 
+    have term_n := Classical.choose scb_term
 
-    let origin_list : List ((trg : RTrigger obs.toLaxObsolescenceCondition kb.rules) × Fin trg.val.mapped_head.length) := by sorry
+
+    let origin_list : List ((trg : RTrigger obs.toLaxObsolescenceCondition kb.rules) × Fin trg.val.mapped_head.length) := scb.get_origin_list term_n (List.range' 1 term_n) rfl sorry
 
     let init_ccn : CoreChaseNode kb.rules := {
               fs := kb.db.toFactSet
@@ -793,8 +451,6 @@ theorem ex_endo_hom  (cb : CoreChaseBranch kb) (cn : CoreChaseNode kb.rules)
               }
 
   /-
-  computes node list
-
     origin_list = [o1, o2, o3]
 
     cn1 = generateNextCoreChaseBranchElement_usingTrigger init_ccn o1
@@ -802,11 +458,9 @@ theorem ex_endo_hom  (cb : CoreChaseBranch kb) (cn : CoreChaseNode kb.rules)
     cn3 = generateNextCoreChaseBranchElement_usingTrigger cn2 o1
 
     node_list = [init_ccn cn1, cn2, cn3]
-
-
   -/
 
-  let node_list := foldl_save_hist_opt_nodup origin_list init_ccn generateNextCoreChaseBranchElement_usingTrigger_only_active_opt
+  let node_list := foldl_save_hist_opt_nodup origin_list init_ccn generateNextCoreChaseBranchElement_opt
 
     let new_ccb : CoreChaseBranch kb := {
 
@@ -815,7 +469,7 @@ theorem ex_endo_hom  (cb : CoreChaseBranch kb) (cn : CoreChaseNode kb.rules)
       database_first := by
         rw [PossiblyInfiniteList.get?_from_list, ← List.head?_eq_getElem?]
         exact foldl_save_hist_opt_nodup_head_eq
-          origin_list init_ccn generateNextCoreChaseBranchElement_usingTrigger_only_active_opt
+          origin_list init_ccn generateNextCoreChaseBranchElement_opt
 
       triggers_active := by
         intro n before before_eq after after_eq
@@ -823,6 +477,7 @@ theorem ex_endo_hom  (cb : CoreChaseBranch kb) (cn : CoreChaseNode kb.rules)
         exists (after.origin.get (Option.isSome_iff_ne_none.mpr after_origin_some))
         constructor
         exact Option.get_mem (Option.isSome_iff_ne_none.mpr after_origin_some)
+
         sorry
 
       triggers_exist := by
@@ -901,8 +556,6 @@ theorem ex_endo_hom  (cb : CoreChaseBranch kb) (cn : CoreChaseNode kb.rules)
       exists buildCoreChaseBranchFromChaseBranch scb scb_term
       have := buildCoreChaseBranchFromChaseBranch_terminates scb scb_term
       grind
-
-
 
   -- brauchen wir kb.det ?
   theorem main_lhs (ccb : CoreChaseBranch kb) (kb_det : kb.isDeterministic) : (∃ (fs : FactSet sig), fs.finite ∧ fs.universallyModelsKb kb) → ccb.terminates' := by
@@ -1001,6 +654,7 @@ theorem ex_endo_hom  (cb : CoreChaseBranch kb) (cn : CoreChaseNode kb.rules)
 
       -- the set of indices in the scb where f appears in scn.facts
       let Ix := fun (n : Nat) => U ⊆ ((scb.branch.get? n).get (scb_all_some n)).facts
+      -- das gilt nicht xD F in den chat, können wir trotzdem dem hom constructen ?
       have Ix_non_empty : ∃ (n : Nat), Ix n := by
         simp only [Ix]
         apply Classical.byContradiction
@@ -1046,57 +700,24 @@ theorem ex_endo_hom  (cb : CoreChaseBranch kb) (cn : CoreChaseNode kb.rules)
 
     have ex_An_core : ∃ (An_core : FactSet sig), An_core.isWeakCore ∧ An_core.homSubset An := An.exists_weak_core_for_finite_set An_fin
 
+    rcases ex_An_core with ⟨An_core, An_core_c, An_core_homsub⟩
 
-
-    have psc : PseudoCoreChaseBranch kb := {
-      branch := PossiblyInfiniteList.from_list (scb.branch.prefixUpTo n_max)
-      database_first := by
-        have dbf := scb.database_first
-        rw [PossiblyInfiniteList.head_eq] at dbf
-        unfold PossiblyInfiniteList.get? InfiniteList.get at dbf
-        unfold PossiblyInfiniteList.prefixUpTo List.filterMap
-        simp only [PossiblyInfiniteList.get?_from_list]
-        split
-        next x heq =>
-          rw [List.range_eq_nil] at heq
-          contradiction
-        next lst n1 n1l heq =>
-          split
-          next =>
-            grind
-          next opt cn cn_eq =>
-            simp only [List.length_cons, Nat.zero_lt_succ, getElem?_pos, List.getElem_cons_zero, Option.some.injEq]
-            have := List.range_head_eq (List.range (n_max + 1)) n_max (List.toList_toArray)
-            have n1_eq : n1 = 0 := by grind
-            subst n1
-            rw [dbf, Option.some_inj] at cn_eq
-            exact Eq.symm cn_eq
-
-      triggers_active := by
-        intro n before before_eq after after_eq
-
-        have := scb.triggers_active n before sorry after sorry
-        exact this
-
+    let ccb_with_An_core : CoreChaseBranch kb := {
+      branch := PossiblyInfiniteList.from_list [{
+        fs := An_core
+        fs_fin := by sorry
+        core := An_core
+        is_core := An_core_c
+        core_sse := FactSet.homSubset_refl An_core
+        origin := none
+        fs_contains_origin_result := by simp
+      }]
+      database_first := sorry
+      triggers_active := sorry
       triggers_exist := sorry
       fairness := sorry
-      last_index := n_max
-      terminates_at := by
-        intro n gt
-        constructor
-        unfold PossiblyInfiniteList.prefixUpTo
-        sorry
-        sorry
-
-
-
-
-      core_node := sorry
-      core_node_eq := sorry
-
     }
-
-    have ex_ccb_with_An_core : ∃ (ccb_with_An_core : CoreChaseBranch kb) (m : Nat), ((ccb_with_An_core.branch.infinite_list m).get sorry).core.homSubset An := by sorry
+    --have ex_ccb_with_An_core : ∃ (ccb_with_An_core : CoreChaseBranch kb) (m : Nat), ((ccb_with_An_core.branch.infinite_list m).get sorry).core.homSubset An := by sorry
 
     -- 11.
     -- core calc only necc after fin steps
